updates

Jax/Jatlx.lean
@@ -20,198 +20,832 @@
      only one variable on lhs, one expression on right
    - 
 -/
-/------------------------- Syntax of Core ATL -----------------------------------/
 
-/-
-inductive scalar_exp :=
-| Sconst :  real -> scalar_exp
-| SVar : var -> scalar_exp
-| SAdd : scalar_exp -> scalar_exp -> scalar_exp
-| SMult : scalar_exp -> scalar_exp -> scalar_exp
-| SSub : scalar_exp -> scalar_exp -> scalar_exp
-| SDiv : scalar_exp -> scalar_exp -> scalar_exp
-| SPrimFun : List scalar_exp -> scalar_exp
-| SAccess : var -> List ind_exp -> scalar_exp
-inductive atl_exp :=
-| EScalar : scalar_exp -> atl_exp
-| ESum : var -> ind_exp -> ind_exp -> atl_exp -> atl_exp
-| EGen : var -> ind_exp -> ind_exp -> atl_exp -> atl_exp
-| EGuard : pred -> atl_exp -> atl_exp
-| ELet : var -> atl_exp -> atl_exp -> atl_exp-/
-/----------------ATL Syntax in Single-Static-Assignment Form---------------------/
-def real := Nat
-inductive stmt_var := stmtV : var → Nat → stmt_var
+/-************** ATL Syntax in Single-Static-Assignment Form *******************-/
+inductive stmt_var
+| stmtV : String → Nat → stmt_var
 /- since ATL is in normal form, index variables can be standardized into only 4 possible cases -/
-inductive ind_var := 
-| genIV : Nat → ind_var
-| sumIV : Nat → ind_var
-| sumIV1 : Nat → ind_var
-| sumIV2 : Nat → ind_var
+inductive ind_var
+| gen : Nat → ind_var
+| sums : Nat → ind_var
+| sum0 : Nat → ind_var
+| sum1 : Nat → ind_var
 
-inductive ind_exp :=
-| IVar : ind_var → ind_exp
-| IConst : real → ind_exp
-| IAdd : ind_exp → ind_exp → ind_exp
-| IMult : ind_exp → ind_exp → ind_exp 
-| ISub : ind_exp → ind_exp → ind_exp
-| IDiv : ind_exp → ind_exp → ind_exp 
-| ICeilDiv : ind_exp → ind_exp → ind_exp
-| IMod : ind_exp → ind_exp → ind_exp 
-inductive pred :=
-| PTrue
-| PFalse
-| PEq : ind_exp → ind_exp → pred
-| PLeq : ind_exp → ind_exp → pred
-| PLe : ind_exp → ind_exp → predicatae
-| PAnd : pred → pred → pred
+inductive ind_exp 
+| var : ind_var → ind_exp
+| const : Nat → ind_exp
+| add : ind_exp → ind_exp → ind_exp
+| mult : ind_exp → ind_exp → ind_exp 
+| sub : ind_exp → ind_exp → ind_exp
+| div : ind_exp → ind_exp → ind_exp 
 
+inductive pred 
+| true
+| false
+| eq : ind_exp → ind_exp → pred
+| le : ind_exp → ind_exp → pred
+| lt : ind_exp → ind_exp → pred
+| and : pred → pred → pred
+| or : pred → pred → pred
 
-inductive stmt_var_acc :
-| stmtVA : stmt_var → List ind_var → stmt_var_acc
-
+inductive binPrim
+| add
+| mult
+| sub
+| div
+inductive uniPrim
+| neg
 /- scalar expressions -/
-inductive exp := 
-| EConst : real → exp
-| EBinOp : 
-  pred → stmt_var_acc → binPrim
-  pred → stmt_var_acc → exp
-| EUniOp : 
-  pred → uniPrim → stmt_var_acc → exp
-| EBinTensorSum : 
-  List Nat → List Nat → List ind_var →
-  pred → stmt_var_acc → stmt_var_acc → exp
-| EUniTensorSum :
-  List ind_var → List ind_var →
-  pred → stmt_var_acc → exp
+inductive exp  
+| const : Nat → exp
+| binOp : 
+  pred → stmt_var → binPrim →
+  pred → stmt_var → exp
+| uniOp : 
+  pred → uniPrim → stmt_var → exp
+| binTenSum : 
+  List Nat → List Nat → List Nat →
+  pred → stmt_var → stmt_var → exp
+| uniTenSum :
+  List Nat → List Nat →
+  pred → stmt_var → exp
+
+inductive tenVal
+| val : List Nat → List Nat → tenVal
+
+inductive genIndBound
+| const : Nat → genIndBound
+| var : stmt_var → Nat → genIndBound
+| max : stmt_var → Nat → stmt_var → Nat → genIndBound
 /- tensor expession -/
-inductive genTenExp :=
-| GScalar : exp → genTenExp
-| Gen : Nat → genTenExp → genTenExp /- shape and expression for each entry -/
-inductive unitTenExp := 
-| TGen : genTenExp → unitTenExp
-| TVar : stmt_var → unitTenExp
+inductive unitTenExp  
+| gen : List genIndBound → exp → unitTenExp
+| var : stmt_var → unitTenExp
+| val : tenVal → unitTenExp
+inductive tenStmt
+| stmt : stmt_var → unitTenExp → tenStmt
+| skip
 inductive tenExp
-| TLetList : List (stmt_var * unitTenExp) * stmt_var → tenExp
+| letList : List tenStmt → stmt_var → tenExp
 /- functions taking tensors as input and returns a tensor, SSA without structs -/
 /- list of input vars (vars that don't occur in lhs before they occur in rhs) 
    and list of statements -/
-inductive tenFunc :=
-| TFunc : List stmt_var -> tenExp -> tenFunc
+inductive tenFunc 
+| func : List stmt_var → tenExp → tenFunc
 
-/---------------- Jaxpr and Lowering it to ATL ---------------------/
-inductive jaxpr_body :=
-| JLetList : List (stmt_var * var * List stmt_var) * stmt_var → jaxpr_body
-inductive jaxpr := 
-| JFunc : List stmt_var → jaxpr_body -> jaxpr
+/-******************** Jaxpr and Lowering it to ATL ********************-/
+inductive jStmt
+| stmt : stmt_var → String → List stmt_var → jStmt
+| skip
+inductive jaxpr_body 
+| letList : List jStmt → stmt_var → jaxpr_body
+inductive jaxpr  
+| func : List stmt_var → jaxpr_body → jaxpr
 
-def subst_lst_gen paras args suf :=
+def subst_lst_gen paras args (suf : Nat) :=
   match paras, args with
-  | [], _ → []
-  | _, [] → []
-  | (stmtV para sufp) :: rstparas, 
-    arg :: rstargs →
-    ((stmtV para suf), TVar arg) :: 
+  | [], _ => []
+  | _, [] => []
+  | (stmt_var.stmtV para _) :: rstparas, 
+    arg :: rstargs =>
+    (tenStmt.stmt (stmt_var.stmtV para suf) (unitTenExp.var arg)) :: 
     subst_lst_gen rstparas rstargs suf
 def var_suf_set stVar suf :=
   match stVar with
-  | stmtV var suf' → stmtV var suf
-def suf_update suf stmt :=
-  match stmt with
-  | (varLHS, TVar varRHS) →
-    ((var_suf_set varLHS suf), TVar (var_suf_set varRHS suf))
-  | (svar, gen indList e) →
-    match e with
-    | EConst c → e
-    | EBinOp p1 (stmtVA var1 accLst1) op
-            p2 (stmtVA var2 accLst2) →
-      EBinOp p1 (stmtVA (var_suf_set var1 suf) accLst1) op
-            p2 (stmtVA (var_suf_set var2 suf) accLst2) 
-    | EUniOp p f (stmtVA var accLst) →
-      EUniOp p f (stmtVA (var_suf_set var suf) accLst)
-    | EBinTensorSum indLst1 indLst2 indLst3 p
-                   (stmtVA var1 accLst1)
-                   (stmtVA var2 accLst2) →
-      EBinTensorSum indLst1 indLst2 indLst3 p
-                   (stmtVA (var_suf_set var1 suf) accLst1)
-                   (stmtVA (var_suf_set var2 suf) accLst2)
-    | EUniTensorSum indLst1 indLst2 p
-                   (stmtVA var1 accLst1) →
-      EUniTensorSum indLst1 indLst2 p
-                   (stmtVA (var_suf_set var1 suf) accLst1)
-def inline_prims stmts env var_suf :=
+  | stmt_var.stmtV var _ => stmt_var.stmtV var suf
+def exp_suf_update (suf : Nat) : exp → exp
+  | exp.const c => exp.const c
+  | exp.binOp p1 var1 op
+               p2 var2 =>
+    exp.binOp p1 (var_suf_set var1 suf) op
+               p2 (var_suf_set var2 suf)
+  | exp.uniOp p f var =>
+    exp.uniOp p f (var_suf_set var suf)
+  | exp.binTenSum indLst1 indLst2 indLst3
+                   p var1 var2 =>
+    exp.binTenSum indLst1 indLst2 indLst3 p
+                   (var_suf_set var1 suf) (var_suf_set var2 suf)
+  | exp.uniTenSum indLst1 indLst2 p var =>
+    exp.uniTenSum indLst1 indLst2 p (var_suf_set var suf)
+def suf_update suf 
+  | tenStmt.stmt varLHS (unitTenExp.var varRHS) =>
+    tenStmt.stmt (var_suf_set varLHS suf) (unitTenExp.var (var_suf_set varRHS suf))
+  | tenStmt.stmt svar (unitTenExp.gen indList e) =>
+    tenStmt.stmt (var_suf_set svar suf) (unitTenExp.gen indList (exp_suf_update suf e))
+  | tenStmt.stmt svar (unitTenExp.val val) =>
+    tenStmt.stmt svar (unitTenExp.val val)
+  | tenStmt.skip => tenStmt.skip
+def inline_prims stmts (env : String → tenFunc) (var_suf : Nat) :=
   match stmts with
-  | [] → []
-  | (target_var, prim_name, arg_vars) :: rst →
+  | [] => []
+  | jStmt.stmt target_var prim_name arg_vars :: rst =>
     match env prim_name with
-    | TFunc inp_vars (TLetList fstmts (stmtV outName outSuf)) →
+    | tenFunc.func inp_vars (tenExp.letList fstmts (stmt_var.stmtV outName _)) =>
       subst_lst_gen inp_vars arg_vars var_suf ++
-      (map (suf_update var_suf) fstmts) ++
-      (target_var, TVar (stmtV outName var_suf)) ::
+      (List.map (suf_update var_suf) fstmts) ++
+      tenStmt.stmt target_var (unitTenExp.var (stmt_var.stmtV outName var_suf)) ::
         inline_prims rst env (1 + var_suf)
+  | jStmt.skip :: rst => tenStmt.skip :: inline_prims rst env var_suf
 /- transform a jaxpr into an ATL, by inlining primitives from environment -/
 def body_trans env body :=
   match body with
-  | JLetList stmts out_var →
-    FLetList (inline_prims stmts env 1) out_var
+  | jaxpr_body.letList stmts out_var =>
+    tenExp.letList (inline_prims stmts env 1) out_var
 def jax_to_ATL p env :=
   match p with
-  | JFunc inp_vars body → 
-    func inp_vars (body_trans env body)
+  | jaxpr.func inp_vars body => 
+    tenFunc.func inp_vars (body_trans env body)
 
-/----------------ATL Semantics in Single-Static-Assignment Form---------------------/
+/-********************* ATL Semantics in Single-Static-Assignment Form ********************-/
 /- given statement list and input environment, 
    return final environment after statements execute -/
-def empty_env := []
-def update_env env para arg :=
-  fun x → if x = para then arg else env x
-def update_env_star env paras args :=
+
+/- Helper Functions for Updating Index Variable Environment -/
+def ivar_env := ind_var → Nat
+def empty_ienv := fun (_ : ind_var) => 0
+def ivar_eq
+  | ind_var.gen a, ind_var.gen b => a == b
+  | ind_var.sums a, ind_var.sums b => a == b
+  | ind_var.sum0 a, ind_var.sum0 b => a == b
+  | ind_var.sum1 a, ind_var.sum1 b => a == b
+  | _, _ => false
+def update_ienv (env : ivar_env) (para : ind_var) (arg : Nat) :=
+  fun x => if ivar_eq x para then arg else env x
+def update_ienv_star env (paras : List ind_var) (args : List Nat) :=
   match paras, args with
-  | _, [] → env
-  | [], _ → env
-  | para :: paras', arg :: args' →
-    update_env_star (update_env env para arg) paras' args'
+  | _, [] => env
+  | [], _ => env
+  | para :: paras', arg :: args' =>
+    update_ienv_star (update_ienv env para arg) paras' args'
 /- https://www.leanprover.cn/mp-lean-zh/main/05_syntax.html -/
-notation (name := env_update) para:arg "!->" arg:arg ";" env:arg =>
-  (update_env env para arg)
-notation (name := env_updates) paras:arg "!->*" args:arg ";" env:arg =>
-  (update_env_star env paras args)
+notation (name := env_update) para:arg "!->i" arg:arg ";" env:arg =>
+  (update_ienv env para arg)
+notation (name := env_updates) paras:arg "!->i*" args:arg ";" env:arg =>
+  (update_ienv_star env paras args)
 
-def gen_list_h ind_var length e env :=
+/- Helper Functions for Updating Statement Variable Environment -/
+def svar_env := stmt_var → tenVal
+def empty_senv : svar_env :=
+  fun _ => tenVal.val [] []
+def svar_eq
+  | stmt_var.stmtV str1 n1, stmt_var.stmtV str2 n2 =>
+    Bool.and (str1 == str2) (n1 == n2)
+def update_senv {A} (env : stmt_var → A) (para : stmt_var) (arg : A) :=
+  fun x => if svar_eq x para then arg else env x
+def update_senv_star {A} (env : stmt_var → A) (paras : List stmt_var) (args : List A) :=
+  match paras, args with
+  | _, [] => env
+  | [], _ => env
+  | para :: paras', arg :: args' =>
+    update_senv_star (update_senv env para arg) paras' args'
+notation (name := senv_update) para:arg "!->s" arg:arg ";" env:arg =>
+  (update_senv env para arg)
+notation (name := senv_updates) paras:arg "!->s*" args:arg ";" env:arg =>
+  (update_senv_star env paras args)
+/- Helper Functions for Working with Indices and Predicates -/
+def ind_incr ivar :=
+  match ivar with
+  | ind_var.gen n => 
+    ind_var.gen (Nat.succ n)
+  | ind_var.sums n => 
+    ind_var.sums (Nat.succ n)
+  | ind_var.sum1 n => 
+    ind_var.sum1 (Nat.succ n)
+  | ind_var.sum0 n => 
+    ind_var.sum0 (Nat.succ n)
+def sum_ind_incr bound_s bound1
+  | ind_var.gen n => 
+    ind_var.gen (Nat.succ n)
+  | ind_var.sums n => 
+    if bound_s < n then ind_var.sum1 0
+    else ind_var.sums (Nat.succ n)
+  | ind_var.sum1 n => 
+    if bound1 < n then ind_var.sum0 0
+    else ind_var.sum1 (Nat.succ n)
+  | ind_var.sum0 n => 
+    ind_var.sum0 (Nat.succ n)
+def eval_ind ie (env : ivar_env) :=
+  match ie with
+  | ind_exp.var ivar => env ivar
+  | ind_exp.const c => c
+  | ind_exp.add ie1 ie2 => 
+    (eval_ind ie1 env) + (eval_ind ie2 env) 
+  | ind_exp.mult ie1 ie2 =>
+    (eval_ind ie1 env) * (eval_ind ie2 env)
+  | ind_exp.sub ie1 ie2 => 
+    (eval_ind ie1 env) - (eval_ind ie2 env) 
+  | ind_exp.div ie1 ie2 => 
+    (eval_ind ie1 env) / (eval_ind ie2 env) 
+def eval_pred_bool p env :=
+  match p with
+  | pred.true => true
+  | pred.false => false
+  | pred.eq ie1 ie2 => 
+    (eval_ind ie1 env) == (eval_ind ie2 env)
+  | pred.le ie1 ie2 => 
+    (eval_ind ie1 env) ≤ (eval_ind ie2 env)
+  | pred.lt ie1 ie2 => 
+    (eval_ind ie1 env) < (eval_ind ie2 env)
+  | pred.and p1 p2 => 
+    if eval_pred_bool p1 env 
+    then eval_pred_bool p2 env else false
+  | pred.or p1 p2 => 
+    if eval_pred_bool p1 env 
+    then true else eval_pred_bool p2 env
+def eval_pred p env :=
+  match eval_pred_bool p env with
+  | true => 1
+  | false => 0
+/- Evaluating Scalar Expressions -/
+/- recursively update the three lists, decrement them, and the expression
+  we have below is the expression for each iteration. The arguments
+  ind_lst* correspond to the exact state of the counter -/
+def decr_lst
+  | [] => []
+  | 0 :: lst' => 0 :: (decr_lst lst')
+  | Nat.succ n :: lst' => n :: lst'
+/- true if all zeros or empty list -/
+def is_all_zeros
+  | [] => true
+  | 0 :: lst' => is_all_zeros lst'
+  | Nat.succ _ :: _ => false 
+
+
+/-
+def sum_2lst ind_lst1 ind_lst2 e env :=
+  let summand := (eval_var_acc e 
+  (var_lst1 !->i* ind_lst1; 
+  (var_lst2 !->i* ind_lst2; env)))
+  match is_all_zeros ind_lst1, is_all_zeros ind_lst2 with
+  | false, _ => summand + (sum_2lst (decr_lst ind_lst1) ind_lst2 e env)
+  | true, false => summand + (sum_2lst ind_lst1 (decr_lst ind_lst2) e env)
+  | true, true => summand
+def sum_3lst ind_lst1 ind_lst2 ind_lst3 e env :=
+  let summand := (eval_var_acc e 
+  (var_lst1 !->i* ind_lst1; 
+  (var_lst2 !->i* ind_lst2; 
+  (var_lst3 !->i* ind_lst3; env))))
+  match is_all_zeros ind_lst1, is_all_zeros ind_lst2, is_all_zeros ind_lst3 with
+  | false, _, _ => summand + (sum_3lst (decr_lst ind_lst1) ind_lst2 ind_lst3 e env)
+  | true, false, _ => summand + (sum_3lst ind_lst1 (decr_lst ind_lst2) ind_lst3 e env)
+  | true, true, false => summand + (sum_3lst ind_lst1 ind_lst2 (decr_lst ind_lst3) e env)
+  | true, true, true => summand
+-/
+def ten_val_acc (shape : List Nat) (content : List Nat) (ind_lst : List Nat) begin_ptr end_ptr :=
+  match shape, ind_lst with
+  | [], [] => content.getD begin_ptr 0
+  | n :: rst_shape, i :: rst_ind_lst =>
+    let one_slice := (List.length content) / n
+    let new_begin := one_slice * i
+    let new_end := one_slice * (1 + i)
+    ten_val_acc rst_shape content rst_ind_lst new_begin new_end
+  | _, _ => 0 /- other cases impossible -/
+def access (senv : svar_env) (ienv : ivar_env) var (acc_lst : List ind_var) :=
+  match senv var with
+  | tenVal.val shape content =>
+    ten_val_acc shape content 
+      (List.map ienv acc_lst) 0 (List.length content)
+def bin_op_app op (n1 n2 : Nat) :=
+  match op with
+  | binPrim.add => n1 + n2
+  | binPrim.sub => n1 - n2
+  | binPrim.mult => n1 * n2
+  | binPrim.div => n1 / n2
+def uni_op_app op (n : Nat) :=
+  match op with
+  | uniPrim.neg => 0 - n
+def sum_tensor_h (sum_inds : List Nat) f senv ienv cur_ind (incr : ind_var -> ind_var) :=
+  match sum_inds with
+  | []  => f senv ienv
+  | n :: rst_sum_inds =>
+    sum_list cur_ind n f ienv senv rst_sum_inds incr
+where sum_list (cur_ind : ind_var) length (f : svar_env -> ivar_env -> Nat) 
+(ienv : ivar_env) (senv : svar_env) (sum_inds : List Nat) (incr: ind_var -> ind_var) :=
   match length with
-  | 0 → []
-  | S n → 
-    (gen_tensor e (ind_var !-> n ; env)) ::
-    gen_list_h ind_var n e env
-def gen_list ind_var length e env :=
-  rev (gen_list_h ind_var length e env)
-/- gen tensor is gen list applied many times-/
-def gen_tensor_h e env cur_ind :=
-  match e with
-  | GScalar → eval_exp e env
-  | Gen n e' →
-    (gen_list cur_ind n 
-      (gen_tensor rst_shape e env (1 + cur_ind)) env)
+  | 0 => 0
+  | Nat.succ n => 
+    (sum_list cur_ind n f ienv senv sum_inds incr) +
+    (sum_tensor_h sum_inds f senv (cur_ind !->i n ; ienv) (incr cur_ind) incr)
+def sum_1tens sum_ind sum_ind_tens p var ind_acc senv ienv :=
+  let f := fun senv ienv => 
+           if eval_pred_bool p ienv 
+           then access senv ienv var ind_acc
+           else 0
+  let incr := sum_ind_incr (List.length sum_ind) 0
+  sum_tensor_h (sum_ind ++ sum_ind_tens) f senv ienv (ind_var.sums 0) incr
+def sum_2tens sum_ind1 sum_ind2 sum_ind3 p var1 ind_acc1 var2 ind_acc2 senv ienv :=
+  let f := fun senv ienv => 
+           if eval_pred_bool p ienv then
+           (access senv ienv var1 ind_acc1) * (access senv ienv var2 ind_acc2)
+           else 0
+  let incr := sum_ind_incr (List.length sum_ind1) (List.length sum_ind2)
+  sum_tensor_h (sum_ind1 ++ sum_ind2 ++ sum_ind3) f senv ienv (ind_var.sums 0) incr
+def iota 
+  | 0 => []
+  | Nat.succ n =>  (iota n) ++ [n]
+def eval_exp (senv : svar_env) (ienv : ivar_env) (gen_ind_acc : List ind_var) : exp → Nat
+  | exp.const c => c
+  | exp.binOp p1 var1 op p2 var2 =>
+    let arg1 := if eval_pred_bool p1 ienv
+                then access senv ienv var1 gen_ind_acc 
+                else 0 
+    let arg2 := if eval_pred_bool p2 ienv
+                then access senv ienv var2 gen_ind_acc
+                else 0 
+    bin_op_app op arg1 arg2
+  | exp.uniOp p f var =>
+    if eval_pred_bool p ienv
+    then uni_op_app f (access senv ienv var gen_ind_acc)
+    else 0
+  | exp.binTenSum n0 n1 ns p var0 var1 =>
+    let ind_acc0 := List.map ind_var.sums (iota (List.length n0))
+    let ind_acc1 := List.map ind_var.sum1 (iota (List.length n1))
+    sum_2tens n0 n1 ns p var0 ind_acc0 var1 ind_acc1 senv ienv
+  | exp.uniTenSum n nS p var =>
+    let ind_acc := List.map ind_var.sums (iota (List.length n))
+    sum_1tens n nS p var ind_acc senv ienv
     
-def gen_tensor e env := gen_tensor_h e env 0
-def eval_texp e env := 
-  match e with
-  | TGen e' →
-    gen_tensor e' env
-  | TVar v →
-    (env v)
-def eval_stmts stmts env :=
-  match stmts with
-  | [] → env
-  | (x, e) :: rst_stmts →
-    let new_env = x !-> (eval_texp e env) ; env in
-    eval_stmts rst_stmts new_env
+/- Evaluating Tensor Expressions -/
+/-  
+/- environment gives 0 by default, so shape list can be shrunk and information not lost-/
+def gen_tensor_h (shape counter : List Nat) (e : exp) senv ienv :=
+  let element := (eval_exp senv ((gen_ind_lst (List.length counter)) !->i* counter; ienv) e)
+  match counter with
+  | [] => [element]
+  | 0 :: lst' => gen_tensor_h shape lst' e senv ienv
+  | Nat.succ n :: lst' => 
+    (gen_tensor_h shape (n :: lst') e senv ienv) ++ [element]
+  
+/- turn the last index to front -/
+def gen_tensor shape e senv := 
+  tenVal.TVal shape (gen_tensor_h (List.reverse shape) (List.reverse shape) e senv empty_ienv)
+-/
 
-List (stmt_var * unitTenExp) 
+def gen_ind_lst
+  | 0 => []
+  | Nat.succ n =>  (gen_ind_lst n) ++ [ind_var.gen n]
+
+/- gen tensor is gen list applied many times-/
+def gen_tensor_h (shape : List Nat) e senv ienv cur_ind (gen_ind_lst : List ind_var) :=
+  match shape with
+  | []  => [eval_exp senv ienv gen_ind_lst e]
+  | n :: rst_shape =>
+    gen_list cur_ind n e ienv senv rst_shape gen_ind_lst
+where gen_list cur_ind_var length (e : exp) (ienv : ivar_env) 
+      (senv : svar_env) (shape : List Nat) (gen_ind_lst : List ind_var) :=
+  match length with
+  | 0 => []
+  | Nat.succ n => 
+    (gen_list cur_ind_var n e ienv senv shape gen_ind_lst) ++
+    gen_tensor_h shape e senv (cur_ind_var !->i n ; ienv) (ind_incr cur_ind_var) gen_ind_lst
+
+def gen_tensor shape e senv := 
+  let gen_ind_lst := List.map ind_var.gen (iota (List.length shape))
+  tenVal.val shape (gen_tensor_h shape e senv empty_ienv (ind_var.gen 0) gen_ind_lst)
+def get_shape_tm (senv : svar_env) var :=
+  match senv var with
+  | tenVal.val shape _ => shape
+
+def eval_shape {X} (get_shape : (svar → X) → stmt_var → List Nat) env
+  | [] => []
+  | genIndBound.const n :: rst_shape => n :: (eval_shape get_shape env rst_shape)
+  | genIndBound.var name ind :: rst_shape =>
+    (get_shape env name).getD ind 0 :: (eval_shape get_shape env rst_shape)
+  | genIndBound.max name1 ind1 name2 ind2 :: rst_shape =>
+    let n1 := (get_shape env name1).getD ind1 0
+    let n2 := (get_shape env name2).getD ind2 0
+    max n1 n2 :: (eval_shape get_shape env rst_shape)
+def eval_shape_tm env shape := eval_shape get_shape_tm env shape
+def eval_texp e senv := 
+  match e with
+  | unitTenExp.gen shape e' =>
+    gen_tensor (eval_shape_tm senv shape) e' senv
+  | unitTenExp.var var =>
+    senv var
+  | unitTenExp.val val => val
+/- Evaluating Programs Expressions -/
+/- given start environment, return environment after statements execute -/
+
+def eval_stmts (env : svar_env) :
+  List tenStmt → svar_env
+  | [] => env
+  | (tenStmt.stmt x e) :: rst_stmts =>
+    let new_env := x !->s (eval_texp e env) ; env
+    eval_stmts new_env rst_stmts
+  | tenStmt.skip :: rst_stmts =>
+    eval_stmts env rst_stmts
+
 def eval_prog prog args fenv :=
-  match jaxToATL prog fenv with
-  | func inp_vars (letList stmts out) →
-    eval_stmts stmts (updateEnv empty_env inp_vars args)
- 
+  match jax_to_ATL prog fenv with
+  | tenFunc.func inp_vars (tenExp.letList stmts out) =>
+    (eval_stmts (inp_vars !->s* args ; empty_senv) stmts) out
+/- ************ Small Step Operational Semantics ************* -/
+inductive step_stmt : svar_env × tenStmt →
+                      svar_env × tenStmt → Prop where
+| stp_stmt : ∀ env var exp,
+  val = eval_texp exp env →
+  new_env = var !->s val ; env →
+  step_stmt (env, (tenStmt.stmt var exp)) (new_env, tenStmt.skip)
+inductive step_stmts : svar_env × List tenStmt →
+                       svar_env × List tenStmt → Prop where
+| stp_skip : ∀ env some_stmts,
+  step_stmts (env, tenStmt.skip :: some_stmts) (env, some_stmts)
+| stp_stmts : ∀ env new_env stmt new_stmt some_stmts,
+  step_stmt (env, stmt) (new_env, new_stmt) →
+  step_stmts (env, stmt :: some_stmts) (new_env, new_stmt :: some_stmts)
+inductive step_fun_body : svar_env × tenExp →
+                          svar_env × tenExp → Prop where
+| stp_letList : ∀ env new_env stmts new_stmts out,
+  step_stmts (env,stmts) (new_env, new_stmts) →
+  step_fun_body (env, tenExp.letList stmts out) (new_env, tenExp.letList new_stmts out)
+/-
+take a program and get an absmachine initial state is not
+part of stepping semantics
+
+inductive steps_prog prog args fenv result
+| stps_prog : ∀ inp_vars stmts out final_env,
+  jax_to_ATL prog fenv = tenFunc.func inp_vars (tenExp.letList stmts out) →
+  steps_stmts (inp_vars !->s* args ; empty_senv) stmts final_env →
+  final_env out = result →
+  steps_prog prog args fenv result-/
+/- ************* Type System & Soundness Proof *************** -/
+/- ************* Type Syntax *************** -/
+inductive ty_unitTenExp  
+| gen : List genIndBound → ty_unitTenExp
+| val : List Nat → ty_unitTenExp
+| var : stmt_var → ty_unitTenExp
+
+inductive ty_tenStmt
+| stmt : stmt_var → ty_unitTenExp → ty_tenStmt
+| skip
+
+inductive ty_tenExp
+| letList : List ty_tenStmt → stmt_var → ty_tenExp
+
+inductive ty_tenFunc 
+| func : List stmt_var → ty_tenExp → ty_tenFunc
+
+/- type of an array value is its shape -/
+inductive ty_tenVal
+| val : List Nat → ty_tenVal
+
+inductive ty_jStmt
+| stmt : stmt_var → String → List stmt_var → ty_jStmt
+| skip
+
+inductive ty_jaxpr_body 
+| letList : List ty_jStmt → stmt_var → ty_jaxpr_body
+
+inductive ty_jaxpr  
+| func : List stmt_var → ty_jaxpr_body → ty_jaxpr
+/- ************* Small Step Type Reduction *************** -/
+/- type environment -/
+def ty_env := stmt_var → ty_tenVal
+def empty_tyenv : ty_env :=
+  fun _ => ty_tenVal.val []
+def lift_senv (senv : svar_env) :=
+  fun x => 
+  match senv x with
+  | tenVal.val shape _ => ty_tenVal.val shape
+/- reduction rules -/
+def get_shape_ty (senv : ty_env) var :=
+  match senv var with
+  | ty_tenVal.val shape => shape
+def eval_shape_ty env shape := eval_shape get_shape_ty env shape
+def eval_ty_texp (senv : ty_env) 
+  | ty_unitTenExp.val shape =>
+    ty_tenVal.val shape
+  | ty_unitTenExp.gen shape =>
+    ty_tenVal.val (eval_shape_ty senv shape)
+  | ty_unitTenExp.var var => senv var
+inductive ty_step_stmt : ty_env × ty_tenStmt →
+                         ty_env × ty_tenStmt → Prop where
+| stp_stmt : ∀ env var exp_ty,
+  val = eval_ty_texp env exp_ty →
+  new_env = var !->s val ; env →
+  ty_step_stmt (env, (ty_tenStmt.stmt var exp_ty)) (new_env, ty_tenStmt.skip)
+inductive ty_step_stmts : ty_env × List ty_tenStmt →
+                          ty_env × List ty_tenStmt → Prop where
+| stp_skip : ty_step_stmts (env, ty_tenStmt.skip :: some_stmts) (env, some_stmts)
+| stp_stmts : ∀ env new_env stmt,
+  ty_step_stmt (env, stmt) (new_env, new_stmt) →
+  ty_step_stmts (env, stmt :: some_stmts) (new_env, new_stmt :: some_stmts)
+inductive ty_step_fun_body : ty_env × ty_tenExp →
+                             ty_env × ty_tenExp → Prop where
+| stp_letList : ∀ env new_env stmts new_stmts out,
+  ty_step_stmts (env,stmts) (new_env, new_stmts) →
+  ty_step_fun_body 
+    (env, ty_tenExp.letList stmts out) 
+    (new_env, ty_tenExp.letList new_stmts out)
+inductive ty_step_fun_body_star : ty_env × ty_tenExp →
+                                  ty_env × ty_tenExp → Prop where
+| no_stp : ∀ env ty, ty_step_fun_body_star (env, ty) (env, ty)
+| stps  : ∀ env ty env' ty' env'' ty'', 
+  ty_step_fun_body_star (env, ty) (env', ty') →
+  ty_step_fun_body (env', ty') (env'', ty'') →
+  ty_step_fun_body_star (env, ty) (env'', ty'')
+/- ************* Typing Rules *************** -/
+inductive has_ty_unitTenExp : unitTenExp → ty_unitTenExp → Prop where
+| gen : ∀ gen_tm gen_ty,
+  gen_tm = unitTenExp.gen shape e →
+  gen_ty = ty_unitTenExp.gen shape →
+  has_ty_unitTenExp gen_tm gen_ty
+| var : ∀ var_tm var_ty,
+  var_tm = unitTenExp.var var →
+  var_ty = ty_unitTenExp.var var →
+  has_ty_unitTenExp var_tm var_ty
+| val : ∀ val_tm val_ty,
+  val_tm = unitTenExp.val (tenVal.val shape content) →
+  val_ty = ty_unitTenExp.val shape →
+  has_ty_unitTenExp val_tm val_ty
+inductive has_ty_tenStmt : tenStmt → ty_tenStmt → Prop where
+| stmt : ∀ stmt_tm stmt_ty var_tm var_ty exp_tm exp_ty,
+  stmt_tm = tenStmt.stmt var_tm exp_tm →
+  stmt_ty = ty_tenStmt.stmt var_ty exp_ty →
+  svar_eq var_tm var_ty = true →
+  has_ty_unitTenExp exp_tm exp_ty →
+  has_ty_tenStmt stmt_tm stmt_ty
+def has_ty_stmtLst 
+  | [], [] => True
+  | stmt_tm :: tm_lst, 
+    stmt_ty :: ty_lst =>
+    has_ty_tenStmt stmt_tm stmt_ty ∧
+    has_ty_stmtLst tm_lst ty_lst
+  | _, _ => False
+inductive has_ty_tenExp : tenExp → ty_tenExp → Prop where
+| letList : ∀ letList_tm letList_ty tm_lst ty_lst out_tm out_ty,
+  letList_tm = tenExp.letList tm_lst out_tm →
+  letList_ty = ty_tenExp.letList ty_lst out_ty →
+  svar_eq out_tm out_ty = true →
+  has_ty_stmtLst tm_lst ty_lst → 
+  has_ty_tenExp letList_tm letList_ty
+def svar_lst_eq
+  | [], [] => true
+  | v1 :: lst1, v2 :: lst2 =>
+    if svar_eq v1 v2 then svar_lst_eq lst1 lst2
+    else false
+  | _, _ => false
+inductive has_ty_tenFunc : tenFunc → ty_tenFunc → Prop where
+| func : ∀ func_tm func_ty inps_tm inps_ty body_tm body_ty,
+  func_tm = tenFunc.func inps_tm body_tm →
+  func_ty = ty_tenFunc.func inps_ty body_ty → 
+  svar_lst_eq inps_tm inps_ty →
+  has_ty_tenExp body_tm body_ty →
+  has_ty_tenFunc func_tm func_ty
+
+inductive has_ty_tenVal : tenVal → ty_tenVal → Prop where
+| val : ∀ val_tm val_ty,
+  val_tm = tenVal.val shape content →
+  val_ty = ty_tenVal.val shape →
+  has_ty_tenVal val_tm val_ty
+inductive has_ty_jStmt : jStmt → ty_jStmt → Prop where
+| stmt : ∀ stmt_tm stmt_ty var_tm var_ty 
+           prim_tm prim_ty args_tm args_ty,
+  stmt_tm = jStmt.stmt var_tm prim_tm args_tm →
+  stmt_ty = ty_jStmt.stmt var_ty prim_ty args_ty →
+  svar_eq var_tm var_ty = true →
+  (prim_tm == prim_ty) = true →
+  svar_lst_eq args_tm args_ty →
+  has_ty_jStmt stmt_tm stmt_ty
+def has_ty_jStmtLst 
+  | [], [] => True
+  | stmt_tm :: tm_lst,
+    stmt_ty :: ty_lst =>
+    has_ty_jStmt stmt_tm stmt_ty ∧
+    has_ty_jStmtLst tm_lst ty_lst
+  | _, _ => False
+
+inductive has_ty_jaxpr_body : jaxpr_body → ty_jaxpr_body → Prop where
+| letList : ∀ letList_tm letList_ty 
+              tm_lst ty_lst out_tm out_ty,
+  letList_tm = jaxpr_body.letList tm_lst out_tm →
+  letList_ty = ty_jaxpr_body.letList ty_lst out_ty →
+  svar_eq out_tm out_ty = true →
+  has_ty_jStmtLst tm_lst ty_lst →
+  has_ty_jaxpr_body letList_tm letList_ty
+
+inductive has_ty_jaxpr : jaxpr → ty_jaxpr → Prop where
+| func : ∀ func_tm func_ty inps_tm inps_ty body_tm body_ty,
+  func_tm = jaxpr.func inps_tm body_tm →
+  func_ty = ty_jaxpr.func inps_ty body_ty → 
+  svar_lst_eq inps_tm inps_ty →
+  has_ty_jaxpr_body body_tm body_ty →
+  has_ty_jaxpr func_tm func_ty
+
+inductive is_terminal : tenExp → Prop where
+| is_term : ∀ tm out,
+  tm = tenExp.letList [] out →
+  is_terminal tm
+
+def ty_eq env1 ty1 env2 ty2 :=
+  ∃ env ty, 
+  ty_step_fun_body_star (env1, ty1) (env, ty) ∧
+  ty_step_fun_body_star (env2, ty2) (env, ty)
+/-
+inductive has_type_atl : tenFunc → ty → Prop where
+| T_atl : ∀ body inp_shapes, 
+  type_of_free_vars body = inp_shapes →
+  has_type_atl_body body out_shapes →
+  has_type_atl 
+    (tenFunc.TFunc inp_vars body)
+    (func_ty inp_shapes out_shapes)
+inductive has_type_j_body
+inductive has_type_j : jaxpr → ty → Prop where
+| T_prog : ∀ jbody inp_shapes, 
+  type_of_free_vars jbody = inp_shapes →
+  has_type_jbody jbody out_shapes →
+  has_type_j 
+    (jaxpr.func inp_vars jbody)
+    (func_ty inp_shapes out_shapes) -/
+/- type abs and app for shapes and ranks -/
+/- function type should give info for how to compute a shape when given a list of shapes -/
+/- shapes of inputs and shape of output -/
+/-
+inductive ty 
+| func_ty : List (List Nat) → List Nat → ty
+| val_ty : List Nat → ty
+def type_of_free_vars seen_vars : List (stmt_var × String × List stmt_var) → List (List Nat)
+  | jaxpr_body.JLetList [] out => []
+  | jaxpr_body.JLetList ((var, prim_func, arg_lst) :: stmt_lst) out =>
+    if List.filter seen_vars arg_lst = []
+    type_of_free_vars stmt_lst
+
+    
+theorem progress : eval_prog simple_prog [arg1,arg2,arg3] prim_env = 
+             tenVal.TVal [2,2] [8, 9, 8, 9] := by simp-/
+/- ************* Type Soundness *************** -/
+
+theorem progress : ∀ tm env ty,
+  has_ty_tenExp tm ty →
+  is_terminal tm ∨
+  ∃ env' tm', step_fun_body (env, tm) (env', tm') := by
+  intros tm env ty H
+  cases tm with
+  | letList stmts out =>
+    cases stmts
+    . apply Or.inl; apply is_terminal.is_term ; rfl
+    case cons stmt rst_stmts => 
+      apply Or.inr
+      cases stmt
+      case skip => 
+        exists env, tenExp.letList rst_stmts out
+        apply step_fun_body.stp_letList
+        apply step_stmts.stp_skip
+      case stmt var exp =>
+        exists var !->s (eval_texp exp env) ; env
+        exists tenExp.letList (tenStmt.skip :: rst_stmts) out
+        apply step_fun_body.stp_letList
+        apply step_stmts.stp_stmts
+        apply step_stmt.stp_stmt
+        . rfl
+        . rfl
+  
+theorem preservation : ∀ tm env tm' env' ty,
+  step_fun_body (env, tm) (env', tm') →
+  has_ty_tenExp tm ty →
+  ∃ ty', 
+    has_ty_tenExp tm' ty' ∧
+    ty_eq (lift_senv env) ty (lift_senv env') ty' := by
+  intros tm env tm' env' ty H_step H_ty
+  cases H_step with
+  | stp_letList env env' stmts stmts' out H_stp_stmts =>
+  cases H_stp_stmts with
+  | stp_skip env some_stmts => 
+    cases H_ty with
+    | letList letList_tm letList_ty out_tm out_ty
+              H_tm H_ty H_var_eq H_stmts_ty =>
+      subst_vars
+      cases H_tm
+      cases letList_ty with
+      | nil => contradiction
+      | cons stmt_ty rst_stmts_ty =>
+      exists (ty_tenExp.letList rst_stmts_ty out_ty)
+      apply And.intro
+      . apply has_ty_tenExp.letList <;> try rfl
+        apply H_var_eq
+        cases H_stmts_ty with
+        | intro left right => apply right
+      . 
+      unfold has_ty_stmtLst at H_stmts_ty
+      simp at H_stmts_ty
+      
+
+| letList : ∀ letList_tm letList_ty tm_lst ty_lst out_tm out_ty,
+  letList_tm = tenExp.letList tm_lst out_tm →
+  letList_ty = ty_tenExp.letList ty_lst out_ty →
+  svar_eq out_tm out_ty = true →
+  has_ty_stmtLst tm_lst ty_lst → 
+  has_ty_tenExp letList_tm letList_ty
+
+
+  | stp_stmts env env' stmt new_stmt some_stmts H_stp_stmt => 
+      
+  
+    
+
+
+  cases tm with
+  | letList stmts out =>
+  cases ty with
+  | letList stmts_ty out_ty =>
+  cases stmts with
+  | nil => contradiction
+  | cons stmt rst_stmts =>
+  cases stmts_ty with
+  | nil => contradiction
+  | cons stmt_ty rst_stmts_ty =>
+  cases stmt with
+  | skip =>
+    cases stmt_ty with
+    | skip => 
+      exists (ty_tenExp.letList rst_stmts_ty out_ty)
+      apply And.intro
+      . 
+    | stmt var exp_ty =>
+  | stmt var exp =>
+    cases stmt_ty with
+    | skip =>
+    | stmt var_ty exp_ty =>
+       
+      
+  cases H_step with
+  | stp_letList env env' stmts stmts' out H_stp_stmts =>
+    cases H_stp_stmts with
+    | stp_stmts env env' stmt new_stmt some_stmts H_stp_stmt => 
+      
+    | stp_skip env some_stmts=> 
+    
+    
+stp_stmts : ∀ env new_env stmt new_stmt some_stmts,
+| stp_skip : step_stmts (env, tenStmt.skip :: some_stmts) (env, some_stmts)
+| stp_stmts : ∀ env new_env stmt,
+  step_stmt (env, stmt) (new_env, new_stmt) →
+  step_stmts (env, stmt :: some_stmts) (new_env, new_stmt :: some_stmts)
+
+
+: ∀ env new_env stmts new_stmts out,
+  step_stmts (env,stmts) (new_env, new_stmts) →
+  step_fun_body (env, tenExp.letList stmts out) (new_env, tenExp.letList new_stmts out) 
+/- ********************* Example  **************************** -/
+notation (name := var_name) "!" name:arg => stmt_var.stmtV name 0
+
+def simple_prog :=
+  jaxpr.func [!"x", !"y", !"z"]
+  (jaxpr_body.letList 
+    [(! "a", "add", [!"x",  !"y"]), 
+    (!"b", "add", [! "a",  !"z"])] 
+    (!"b"))
+def add_func :=
+  let p := pred.true
+  let X1 := stmt_var.stmtV (!"x")
+  let X2 := stmt_var.stmtV (!"y")
+  tenFunc.func [!"x",  !"y"]
+    (tenExp.letList [(! "a", unitTenExp.gen [2, 2] 
+                      (exp.binOp p X1 binPrim.add p X2))] (! "a"))
+def arg1 := tenVal.val [2,2] [1, 2, 3, 4]
+def arg2 := tenVal.val [2,2] [6, 5, 2, 1]
+def arg3 := tenVal.val [2,2] [1, 2, 3, 4]
+def prim_env
+  | "add" => add_func
+  | _ => tenFunc.func [] (tenExp.letList [] (! "a"))
+
+theorem eg : eval_prog simple_prog [arg1,arg2,arg3] prim_env = 
+             tenVal.val [2,2] [8, 9, 8, 9] := by
+ /- converting jax to ATL -/
+ unfold eval_prog
+ unfold jax_to_ATL
+ unfold simple_prog
+ unfold body_trans
+ simp
+ unfold inline_prims
+ unfold inline_prims
+ unfold inline_prims
+ unfold prim_env
+ unfold add_func
+ simp
+ unfold suf_update
+ simp
+ unfold exp_suf_update
+ simp
+ unfold var_suf_set
+ simp
+ unfold subst_lst_gen subst_lst_gen subst_lst_gen
+ simp
+ /- running the code -/
+ unfold update_senv_star update_senv_star update_senv_star update_senv_star
+ unfold update_senv
+ unfold eval_stmts update_senv eval_texp
+ simp
+ unfold eval_stmts eval_stmts eval_stmts 
+ unfold eval_stmts eval_stmts eval_stmts eval_stmts eval_stmts
+ unfold update_senv
+ unfold svar_eq
+ simp
+ simp
+ unfold update_senv
+ unfold jax_to_ATL
+ simp
+ unfold body_trans
 /-
 start from let bindings with calls to primitive functions on tensors
 we can replace primitive function f's call to argument variables x_1 to x_n by
